add basic erc20

LiqLeanPolicy/ERC20.lean
@@ -1,9 +1,26 @@
-structure ERC20 where
-  name : String
-  symbol : String
-  totalBalance : Nat
-  delegatedAmount : Nat -- 1000 USDC delegated to Alice
-  deriving DecidableEq
+import LiqLeanPolicy.Basic
 
-def ERC20.totalSupply (self : ERC20) : Nat :=
-  self.totalBalance - self.delegatedAmount
+-- Core token state
+def Balance := Nat
+deriving DecidableEq, Repr, ToString
+
+
+instance [OfNat Nat n] : OfNat Balance n where ofNat := n
+instance : LE Balance where le := Nat.le
+
+structure TokenState where
+  balances : List (Address × Balance)
+
+def getBalance (self : TokenState) (address : Address) : Balance :=
+  match self.balances.find? (fun (addr, _) => addr = address) with
+  | some (_, bal) => bal
+  | none => Nat.zero
+
+def canExternalTransfer (self : TokenState) (transfer : ExternalTransfer) : Prop :=
+  getBalance self transfer.fromAccount.address >= transfer.amount
+
+theorem test_transfer (state : TokenState) (t : ExternalTransfer) :
+  canExternalTransfer state t →
+  t.amount ≤ getBalance state t.fromAccount.address := by
+  intro h
+  exact h
