Main.lean
@@ -1,4 +1,26 @@
-import LiqLeanPolicy
+-- import LiqLeanPolicy
 
-def main : IO Unit :=
-  IO.println s!"Hello, {hello}!"
+-- def main : IO Unit := do
+  -- Create test addresses
+  -- let addr1 := Address.mk "0x1234"
+  -- let addr2 := Address.mk "0x5678"
+
+  -- -- Create test accounts
+  -- let account1 := Account.mk addr1 addr1
+  -- let account2 := Account.mk addr2 addr2
+
+  -- -- Initialize token state with some balances
+  -- let initialState := TokenState.mk [
+  --   (addr1, (1000 : Nat)),
+  --   (addr2, (500 : Nat))
+  -- ]
+
+  -- -- Create a test transfer
+  -- let transfer := ExternalTransfer.mk account1 addr2 100
+
+  -- -- Test balance checking
+  -- let senderBalance := getBalance initialState addr1
+  -- IO.println s!"{addr1}"
+
+def main : IO Unit := do
+IO.println "Hello, World!"
